Refactor

Calculus.v
@@ -14,13 +14,13 @@ with valueType : Type :=
   | HandlerType : computationType -> computationType -> valueType.
 
 Inductive computation : Type :=
-  | CReturn (v : valueExpr)
-  | COp (op : string) (v : valueExpr) (x : string) (c : computation)
+  | CReturn (v : value)
+  | COp (op : string) (v : value) (x : string) (c : computation)
   | CDo (x : string) (c1 c2 : computation) : computation
-  | CIf (b : valueExpr) (c1 c2 : computation) : computation
-  | CApp (v1 : valueExpr) (v2 : valueExpr) : computation
-  | CHandle (e : computation) (h : valueExpr) : computation
-with valueExpr : Type :=
+  | CIf (b : value) (c1 c2 : computation) : computation
+  | CApp (v1 : value) (v2 : value) : computation
+  | CHandle (e : computation) (h : value) : computation
+with value : Type :=
   | VVar (x : string)
   | VTrue
   | VFalse
@@ -30,28 +30,28 @@ with opCase : Type :=
   | OpCase (op : string) (x : string) (k : string) (e : computation).
 
 Scheme computation_mut := Induction for computation Sort Prop
-with valueExpr_mut := Induction for valueExpr Sort Prop
+with value_mut := Induction for value Sort Prop
 with opCase_mut := Induction for opCase Sort Prop.
 
 Fixpoint subst
-  (x : string) (s : valueExpr) (t : computation) :=
+  (x : string) (s : value) (t : computation) :=
   match t with
-  | CReturn v => CReturn (subst_in_valueExpr x s v)
+  | CReturn v => CReturn (subst_in_value x s v)
   | COp op v y c => 
       if eqb_string x y then
-        COp op (subst_in_valueExpr x s v) y c
+        COp op (subst_in_value x s v) y c
       else
-        COp op (subst_in_valueExpr x s v) y (subst x s c)
+        COp op (subst_in_value x s v) y (subst x s c)
   | CDo y c1 c2 => 
       if eqb_string x y then
         CDo y (subst x s c1) c2
       else
         CDo y (subst x s c1) (subst x s c2)
-  | CIf b c1 c2 => CIf (subst_in_valueExpr x s b) (subst x s c1) (subst x s c2)
-  | CApp v1 v2 => CApp (subst_in_valueExpr x s v1) (subst_in_valueExpr x s v2)
-  | CHandle c v => CHandle (subst x s c) (subst_in_valueExpr x s v)
+  | CIf b c1 c2 => CIf (subst_in_value x s b) (subst x s c1) (subst x s c2)
+  | CApp v1 v2 => CApp (subst_in_value x s v1) (subst_in_value x s v2)
+  | CHandle c v => CHandle (subst x s c) (subst_in_value x s v)
   end
-with subst_in_valueExpr (x : string) (s : valueExpr) (t : valueExpr) :=
+with subst_in_value (x : string) (s : value) (t : value) :=
   match t with
   | VVar y => if eqb_string x y then s else t
   | VTrue => VTrue
@@ -67,7 +67,7 @@ with subst_in_valueExpr (x : string) (s : valueExpr) (t : valueExpr) :=
     else
       VHandler xr (subst x s er) (subst_in_opCase x s op)
   end
-with subst_in_opCase (x : string) (s : valueExpr) (t : opCase) :=
+with subst_in_opCase (x : string) (s : value) (t : opCase) :=
   match t with
   | OpCase op y k e => 
     if eqb_string x y || eqb_string x k then
@@ -76,22 +76,11 @@ with subst_in_opCase (x : string) (s : valueExpr) (t : opCase) :=
        OpCase op y k (subst x s e)
   end.
 
-Inductive value : valueExpr -> Prop :=
-  | v_fun : forall x T c,
-      value (VFun x T c)
-  | v_handler : forall xr er op, value (VHandler xr er op)
-  | v_true :
-      value VTrue
-  | v_false :
-      value VFalse.
-
 Reserved Notation "E '\' t '-->' t'" (at level 40).
-
 
 Inductive step : total_map (valueType * valueType) -> computation -> computation -> Prop :=
   | ST_AppAbs : forall E x T2 c v2,
-         value v2 ->
-        E \ CApp (VFun x T2 c) v2 --> subst x v2 c
+      E \ CApp (VFun x T2 c) v2 --> subst x v2 c
   | ST_IfTrue : forall E c1 c2,
       E \ CIf VTrue c1 c2 --> c1
   | ST_IfFalse : forall E c1 c2,
@@ -100,24 +89,19 @@ Inductive step : total_map (valueType * valueType) -> computation -> computation
       E \ c1 --> c1' ->
       E \ CDo x c1 c2 --> CDo x c1' c2
   | ST_DoReturn : forall E x v c,
-      value v ->
       E \ CDo x (CReturn v) c --> subst x v c
   | ST_DoOp : forall E op x v y c1 c2,
-      value v ->
       E \ CDo x (COp op v y c1) c2 --> COp op v y (CDo x c1 c2)
   | ST_Handle1 : forall E c c' h,
       E \ c --> c' ->
       E \ CHandle c h --> CHandle c' h
   | ST_HandleReturn : forall E v xr er op,
-    value v ->
     E \ CHandle (CReturn v) (VHandler xr er op) --> subst xr v er
   | ST_HandleOpEqual : forall E op v y c xr cr x k ch,
-    value v ->
     E \ CHandle (COp op v y c) (VHandler xr cr (OpCase op x k ch)) -->
     subst k (VFun y (snd (E op))
     (CHandle c (VHandler xr cr (OpCase op x k ch)))) (subst x v ch)
   | ST_HandleOpNotEqual : forall E op1 op2 v y c xr cr x k ch,
-    value v ->
     op1 <> op2 ->
     E \ CHandle (COp op1 v y c) (VHandler xr cr (OpCase op2 x k ch)) -->
     COp op1 v y (CHandle c (VHandler xr cr (OpCase op2 x k ch)))
@@ -164,7 +148,7 @@ Inductive has_type : total_map (valueType * valueType) -> context -> computation
 
 where "E '\' Gamma '||-' c '\in' T" := (has_type E Gamma c T)
 
-with has_type_valueExpr : total_map (valueType * valueType) -> context -> valueExpr -> valueType -> Prop :=
+with has_type_value : total_map (valueType * valueType) -> context -> value -> valueType -> Prop :=
   | T_Var : forall E Gamma x T,
       Gamma x = Some T ->
       E \ Gamma |- VVar x \in T
@@ -182,7 +166,7 @@ with has_type_valueExpr : total_map (valueType * valueType) -> context -> valueE
       E \ Gamma |- VHandler xr cr opCase \in 
         (HandlerType (ComputationType A Delta) (ComputationType B Delta'))
 
-where "E '\' Gamma '|-' v '\in' T" := (has_type_valueExpr E Gamma v T)
+where "E '\' Gamma '|-' v '\in' T" := (has_type_value E Gamma v T)
 
 with has_type_opCase : total_map (valueType * valueType) -> context -> string -> opCase -> computationType -> Prop :=
   | T_OpCase : forall E x op k T1 T2 T Gamma c,
